Mica/TinyML/Printer.lean
@@ -147,6 +147,7 @@ partial def printConst : TinyML.Const → String
   | .int n => if n < 0 then s!"({n})" else s!"{n}"
   | .bool b => if b then "true" else "false"
   | .string _ => "\"...\""
+  | .float b => toString (Float.ofBits b)
   | .unit => "()"
 
 partial def printFix (self : Untyped.Binder) (args : List Untyped.Binder) (body : Untyped.Expr) : String :=
